Axioms.v
@@ -1,15 +1,28 @@
 Add LoadPath "." as Top.
 Require Import Top.Definitions.
+Require Import Top.Heap.
 
 Axiom Phi_Seq_Nil_L : forall phi, Phi_Seq Phi_Nil phi = phi.
 Axiom Phi_Seq_Nil_R : forall phi, Phi_Seq phi Phi_Nil = phi.
 Axiom Phi_Par_Nil_R : forall phi, Phi_Par phi Phi_Nil = phi.
 Axiom Phi_Par_Nil_L : forall phi, Phi_Par Phi_Nil phi = phi.
 
-Axiom DeterminismUpToPermutations:
+Axiom EquivalenceUpToPermutations:
   forall (h h' h_: Heap) env rho exp v p,
     H.Equal h' h_ -> (* assume we can prove this for an hypothetical heap:=h_ *)
     H.Equal h h'  -> (* read only p *)
     (h, env, rho, exp) ⇓ (h', v, p) ->
     h' = h_.
 
+Axiom ReadOnlyWalkSameHeap:
+  forall acts_mu1 acts_mu2 h same_h,
+    ReadOnlyPhi (Phi_Par acts_mu1 acts_mu2) ->
+    (Phi_Par acts_mu1 acts_mu2, h) ==>* (Phi_Nil, same_h) ->
+    h = same_h.
+
+Axiom deterministicTcHeap:
+  forall stty1 h stty2 h' acts_mu1 acts_mu2,
+    TcHeap (h, stty1) ->
+    TcHeap (h, stty2) ->
+    (Phi_Par acts_mu1 acts_mu2, h) ==>* (Phi_Nil, h') ->
+    TcHeap (h', Functional_Map_Union stty1 stty2).
